Refinment complete

theories/examples/rwcas.v
@@ -18,15 +18,6 @@ Definition atomic_rwcas : val := λ: <>,
   let: "x" := ref #0 in
   ((λ: "v", atomic_write "x" "v"), (λ: <>, read "x")).
 
-(** Fine-grained, strongly linearizable implementation of a read-write cell. 
-    Read from the cell and attempt to CAS; loop until success *)
-Definition lf_write : val :=
-  rec: "write" "x" "v" :=
-    let: "c" := !"x" in
-    if: CAS "x" "c" "v"
-      then #()
-      else "write" "x" "v".
-
 Definition wf_write : val :=
   λ: "l" "v",
     let: "p" := NewProph in
@@ -34,21 +25,14 @@ Definition wf_write : val :=
     #().
 
 (* Fine-grained implementatiaon of a read-write cell *)
-Definition lf_rwcas : val := λ: <>,
+Definition wf_rwcas : val := λ: <>,
   let: "x" := ref #0 in
-  ((λ: "v", lf_write "x" "v"), (λ: <>, read "x")).
-
-(* Fine-grained implementatiaon of a read-write cell *)
-Definition lf_rwcas : val := λ: <>,
-  let: "x" := ref #0 in
-  ((λ: "v", lf_write "x" "v"), (λ: <>, read "x")).
+  ((λ: "v", wf_write "x" "v"), (λ: <>, read "x")).
 
 (* LP stepping requests. *)
 (* Map the proph id of every failing write to a triple [(id, γₜ, v)]*)
 Definition requestReg := gmap nat (agree (ref_id * gname * Z)).
 Definition requestRegUR := authUR $ gmapUR nat (agreeR (prodO (prodO ref_idO gnameO) ZO)).
-
-Check to_agree_op_inv_L.
 
 Class rwcasG Σ := {
   rwcas_requestUR :: inG Σ requestRegUR;
@@ -289,148 +273,20 @@ Section wf.
         iIntros "!> %vs' -> _ //".
   Qed.
 
-  Lemma lf_atomic_rwcas_refinement : REL wf_rwcas << atomic_rwcas : () → (lrel_int → ()) * (() → lrel_int).
-          
-End wf.
-
-Section atomic_rwcas.
-  Context `{relocG Σ}.
-
-  Lemma read_r E K x (n : Z) t A
-    (Hspec : nclose specN ⊆ E) :
-    x ↦ₛ #n -∗
-    (x ↦ₛ #n -∗ REL t << fill K (of_val #n) @ E : A) -∗ (* TODO: of_val *)
-    REL t << fill K (read #x) @ E : A.
-  Proof.
-    iIntros "Hx Hlog".
-    rel_rec_r. repeat rel_pure_r. rel_load_r.
-    by iApply "Hlog".
-  Qed.
-
-  (* A similar atomic specification for the read fn *)
-  Lemma read_atomic_l R P E K x t A :
-    P -∗
-    □ (|={⊤,E}=> ∃ n : Z, x ↦ #n ∗ R n ∗
-       (x ↦ #n ∗ R n ={E,⊤}=∗ True) ∧
-        (x ↦ #n ∗ R n -∗ P -∗
-            REL fill K (of_val #n) << t @ E : A))
-    -∗ REL fill K (read #x) << t : A.
-  Proof.
-    iIntros "HP #H".
-    rel_rec_l. repeat rel_pure_l. rel_load_l_atomic.
-    iMod "H" as (n) "[Hx [HR Hfin]]". iModIntro.
-    iExists _; iFrame "Hx". iNext.
-    iIntros "Hx".
-    iDestruct "Hfin" as "[_ Hfin]".
-    iApply ("Hfin" with "[Hx HR] HP"). by iFrame.
-  Qed.
-
-  Definition rwcasN : namespace := nroot .@ "rwcas".
-
-  Definition rwcas_inv x x' : iProp Σ :=
-    (∃ n : Z, x ↦ #n ∗ x' ↦ₛ #n)%I.
-
- (* A logically atomic specification for
-     a fine-grained write with a baked in frame. *)
-  Lemma lf_write_atomic_l R P E K x v t A  :
-    P -∗
-    □ (|={⊤,E}=> ∃ n : Z, x ↦ #n ∗ R n ∗
-       ((x ↦ #n ∗ R n ={E,⊤}=∗ True) ∧
-        (x ↦ #v ∗ R n -∗ P -∗
-            REL fill K (of_val #()) << t @ E : A)))
-    -∗ REL fill K (lf_write #x #v) << t : A.
-  Proof.
-    iIntros "HP #H".
-    iLöb as "IH".
-    rel_rec_l. repeat rel_pure_l.
-    iPoseProof "H" as "H2".
-    rel_load_l_atomic.
-    iMod "H" as (n) "[Hx [HR Hrev]]".  iModIntro.
-    iExists #n. iFrame. iNext. iIntros "Hx".
-    iDestruct "Hrev" as "[Hrev _]".
-    iMod ("Hrev" with "[HR Hx]") as "_"; first iFrame.
-    repeat rel_pure_l. rel_cmpxchg_l_atomic.
-    iMod "H2" as (n') "[Hx [HR HQ]]". iModIntro. simpl.
-    destruct (decide (n = n')); subst.
-    - iExists #n'. iFrame. simpl.
-      iSplitR; eauto. { iDestruct 1 as %Hfoo. exfalso. done. }
-      iIntros "_ !> Hx". simpl.
-      iDestruct "HQ" as "[_ HQ]".
-      replace (n' + 1)%Z with (1 + n')%Z by lia. (* TODO :( *)
-      iSpecialize ("HQ" with "[$Hx $HR]").
-      rel_pures_l. by iApply "HQ".
-    - iExists #n'. iFrame. simpl.
-      iSplitL; eauto; last first.
-      { iDestruct 1 as %Hfoo. exfalso. simplify_eq. }
-      iIntros "_ !> Hx". simpl.
-      rel_pures_l.
-      iDestruct "HQ" as "[HQ _]".
-      iMod ("HQ" with "[$Hx $HR]").
-      by iApply "IH".
-  Qed.
-
-  Lemma FG_atomic_write_refinement x x' v1 v2 :
-    inv rwcasN (rwcas_inv x x') -∗ lrel_int v1 v2 -∗
-    REL lf_write #x v1 << atomic_write #x' v2 : lrel_unit.
-  Proof.
-    iIntros "#Hinv".
-    iIntros "(%v & -> & ->)".
-    rel_apply_l
-      (lf_write_atomic_l
-              (fun n => x' ↦ₛ #n)%I
-              True%I); first done.
-    iModIntro. iInv rwcasN as ">Hv" "Hcl". iModIntro.
-    iDestruct "Hv" as (n) "[Hv Hv']".
-    iExists _; iFrame.
-    iSplit.
-    - iIntros "(Hv & Hv')".
-      iApply ("Hcl" with "[-]").
-      iNext. iExists _. iFrame.
-    - iIntros "(Hv & Hv') _".
-      unfold atomic_write. rel_pures_r.
-      rel_store_r.
-      iMod ("Hcl" with "[-]").
-      { iNext. iExists v; iFrame. }
-      rel_values.
-  Qed.
-
-  Lemma read_refinement x x' :
-    inv rwcasN (rwcas_inv x x') -∗
-    REL read #x << read #x' : lrel_int.
-  Proof.
-    iIntros "#Hinv".
-    rel_apply_l
-      (read_atomic_l
-         (fun n => x' ↦ₛ #n)%I
-         True%I); first done.
-    iModIntro. iInv rwcasN as (n) "[>Hv >Hv']" "Hclose".
-    iModIntro.
-    iExists n. iFrame "Hv Hv'".
-    iSplit.
-    - iIntros "(Hv & Hv')". iApply "Hclose".
-      iNext. iExists n. by iFrame.
-    - iIntros "(Hv & Hv') _ /=".
-      rel_apply_r (read_r with "Hv'").
-      iIntros "Hv'".
-      iMod ("Hclose" with "[Hv Hv']"); simpl.
-      { iNext. iExists _. by iFrame. }
-      rel_values.
-  Qed.
-
-  Lemma FG_atomic_rwcas_refinement :
-    ⊢ REL lf_rwcas << atomic_rwcas : () → (lrel_int → ()) * (() → lrel_int).
-  Proof.
+  Lemma wf_atomic_rwcas_refinement : 
+    ⊢ REL wf_rwcas << atomic_rwcas : () → (lrel_int → ()) * (() → lrel_int).
+  Proof using relocG0 rwcasG0 tokenG0 Σ.
     iApply refines_arrow_val.
     iModIntro. iIntros (? ?) "_"; simplify_eq/=.
     rel_rec_l. rel_rec_r.
-    rel_alloc_r v' as "Hv'".
-    rel_alloc_l v as "Hv". simpl.
-
-    (* establishing the invariant *)
-    iAssert (rwcas_inv v v')
-      with "[Hv Hv']" as "Hinv".
-    { iExists 0. by iFrame. }
-    iMod (inv_alloc rwcasN with "[Hinv]") as "#Hinv"; trivial.
+    rel_alloc_l lᵢ as "Hlᵢ".
+    rel_alloc_r lₛ as "Hlₛ".
+    iMod (own_alloc (● map_seq O (to_agree <$> []))) as "[%γ H●]".
+    { by apply auth_auth_valid. }
+    iAssert (rwcas_inv γ lᵢ lₛ) with ("[Hlᵢ Hlₛ H●]") as "Hinv".
+    { iExists 0. iFrame. by rewrite /registry_inv. }
+    iMod (inv_alloc rwcasN with "[Hinv]") as "#Hinv".
+    { done. }
 
     (* TODO: here we have to do /exactly/ 4 steps.
        The next step will reduce `(Val v1, Val v2)` to `Val (v1, v2)`,
@@ -438,19 +294,11 @@ Section atomic_rwcas.
     do 4 rel_pure_r. do 4 rel_pure_l.
     iApply refines_pair.
     - iApply refines_arrow_val.
-      iModIntro. iIntros (? ?) "Hrel". rel_seq_l; rel_seq_r.
-      iApply (FG_atomic_write_refinement with "Hinv"). iFrame.
+      iModIntro. iIntros (? ?) "(%v & -> & ->)". rel_seq_l; rel_seq_r.
+      iApply (write_refinement with "Hinv").
     - iApply refines_arrow_val.
       iModIntro. iIntros (? ?) "_". rel_seq_l; rel_seq_r.
       iApply (read_refinement with "Hinv").
   Qed.
-
-End atomic_rwcas.
-
-Theorem rwcas_ctx_refinement :
-  ∅ ⊨ lf_rwcas ≤ctx≤ atomic_rwcas :
-         () → ((TNat → ()) * (() → TNat)).
-Proof.
-  eapply (refines_sound relocΣ).
-  iIntros (? Δ). simpl. iApply FG_atomic_rwcas_refinement.
-Qed.
+          
+End wf.
